<exercise checkit-seed="0000" checkit-slug="DL2" checkit-title="Laplace Transforms from Definition and Formulas">
  <statement>
      <ol>
      <li>
Compute the Laplace transform of
<m>y = -2 \, t^{4} - 4 \, \cos\left(2 \, t\right) + 4 \, \mathrm{u}\left(t - 1\right) - 4</m> by using a transform table.
      </li>
          <li>
Show why <m>\mathcal{L}\{ 2 \, e^{\left(3 \, t\right)} \}=\frac{2}{s - 3}</m>
using the integral definition of a Laplace transform.
          </li>
      </ol>
  </statement>
  <answer>
      <ol>
          <li>
      <me>
\mathcal{L}\{y\} = -\frac{4 \, s}{s^{2} + 4} + \frac{4 \, e^{\left(-s\right)}}{s} - \frac{4}{s} - \frac{48}{s^{5}}
      </me>
          </li>
          <li>
              <me>
\mathcal{L}\{ 2 \, e^{\left(3 \, t\right)} \}
=\int_0^{\infty} 2 \, e^{\left(3 \, t\right)} e^{-st}\,dt
=\frac{2}{s - 3}
              </me>
          </li>
      </ol>
  </answer>
</exercise>
