<exercise checkit-seed="0009" checkit-slug="DL2" checkit-title="Laplace Transforms from Definition and Formulas">
  <statement>
      <ol>
      <li>
Compute the Laplace transform of
<m>y = 2 \, t^{4} - 4 \, \cos\left(3 \, t\right) + 3 \, \mathrm{u}\left(t - 3\right) + 3</m> by using a transform table.
      </li>
          <li>
Show why <m>\mathcal{L}\{ 3 \, e^{\left(4 \, t\right)} \}=\frac{3}{s - 4}</m>
using the integral definition of a Laplace transform.
          </li>
      </ol>
  </statement>
  <answer>
      <ol>
          <li>
      <me>
\mathcal{L}\{y\} = -\frac{4 \, s}{s^{2} + 9} + \frac{3 \, e^{\left(-3 \, s\right)}}{s} + \frac{3}{s} + \frac{48}{s^{5}}
      </me>
          </li>
          <li>
              <me>
\mathcal{L}\{ 3 \, e^{\left(4 \, t\right)} \}
=\int_0^{\infty} 3 \, e^{\left(4 \, t\right)} e^{-st}\,dt
=\frac{3}{s - 4}
              </me>
          </li>
      </ol>
  </answer>
</exercise>
