<exercise checkit-seed="0007" checkit-slug="Extra2" checkit-title="Clontz Spring 2022 Final">
    <statement>
        <p>
For each of the following ODEs, demonstrate how to find a
general solution (implicit or explicit). If initial value(s) are
given, also show how to find the corresponding particular solution.
        </p>
        <ol>
        <!--  -->
            <li>
                <p>
                    <m>6 \, {y} = -2 \, {y'}</m>
                    <!--  -->
                    , <m>\,\,y(\log\left(2\right)) = -\frac{3}{8}</m>
                    <!--  -->
                    <!--  -->
                </p>
            </li>
        <!--  -->
            <li>
                <p>
                    <m>{y''} + 5 \, {y} = 6 \, {y'}</m>
                    <!--  -->
                    , <m>\,\,y(0) = 4</m>
                    <!--  -->
                    <!--  -->
                    , <m>\,\,y'(0) = 20</m>
                    <!--  -->
                </p>
            </li>
        <!--  -->
            <li>
                <p>
                    <m>9 \, {x} = -{x''}</m>
                    <!--  -->
                    , <m>\,\,y(0) = 3</m>
                    <!--  -->
                    <!--  -->
                    , <m>\,\,y'(0) = -3</m>
                    <!--  -->
                </p>
            </li>
        <!--  -->
            <li>
                <p>
                    <m>-4 \, {y} + 3 \, \delta\left(t - 6\right) = {y'}</m>
                    <!--  -->
                    , <m>\,\,y(0) = -5</m>
                    <!--  -->
                    <!--  -->
                </p>
            </li>
        <!--  -->
            <li>
                <p>
                    <m>-8 \, {y} - {y''} + 6 \, {y'} = 9 \, e^{\left(5 \, t\right)} - 8</m>
                    <!--  -->
                    <!--  -->
                </p>
            </li>
        <!--  -->
            <li>
                <p>
                    <m>{y'} t - 2 \, {y} - \frac{3}{t} = 0</m>
                    <!--  -->
                    , <m>\,\,y(-1) = -3</m>
                    <!--  -->
                    <!--  -->
                </p>
            </li>
        <!--  -->
            <li>
                <p>
                    <m>8 \, y^{3} {y'} + 4 \, t^{2} {y'} - 8 \, t = -8 \, t y</m>
                    <!--  -->
                    , <m>\,\,y(-1) = 1</m>
                    <!--  -->
                    <!--  -->
                </p>
            </li>
        <!--  -->
            <li>
                <p>
                    <m>-3 \, {y'} + 24 \, e^{t} = -15 \, {y}</m>
                    <!--  -->
                    , <m>\,\,y(0) = -1</m>
                    <!--  -->
                    <!--  -->
                </p>
            </li>
        <!--  -->
        </ol>
    </statement>
    <answer>
        <ol>
        <!--  -->
            <li>
                <!--  -->
                <p>
                    <m>{y} = -3 \, e^{\left(-3 \, t\right)}</m>
                </p>
                <!--  -->
                <!--  -->
            </li>
        <!--  -->
            <li>
                <!--  -->
                <p>
                    <m>{y} = 4 \, e^{\left(5 \, t\right)}</m>
                </p>
                <!--  -->
                <!--  -->
            </li>
        <!--  -->
            <li>
                <!--  -->
                <p>
                    <m>{x} = 3 \, \cos\left(3 \, t\right) - \sin\left(3 \, t\right)</m>
                </p>
                <!--  -->
                <!--  -->
            </li>
        <!--  -->
            <li>
                <!--  -->
                <p>
                    <m>{y} = 3 \, e^{\left(-4 \, t + 24\right)} \mathrm{u}\left(t - 6\right) - 5 \, e^{\left(-4 \, t\right)}</m>
                </p>
                <!--  -->
                <!--  -->
            </li>
        <!--  -->
            <li>
                <!--  -->
                <!--  -->
                <p>
                    <m>{y} = k_{2} e^{\left(4 \, t\right)} + k_{1} e^{\left(2 \, t\right)} - 3 \, e^{\left(5 \, t\right)} + 1</m>
                </p>
                <!--  -->
            </li>
        <!--  -->
            <li>
                <!--  -->
                <p>
                    <m>{y} = -4 \, t^{2} - \frac{1}{t}</m>
                </p>
                <!--  -->
                <!--  -->
            </li>
        <!--  -->
            <li>
                <!--  -->
                <p>
                    <m>-2 \, y^{4} - 4 \, t^{2} y + 4 \, t^{2} = \left(-2\right)</m>
                </p>
                <!--  -->
                <!--  -->
            </li>
        <!--  -->
            <li>
                <!--  -->
                <p>
                    <m>y = e^{\left(5 \, t\right)} - 2 \, e^{t}</m>
                </p>
                <!--  -->
                <!--  -->
            </li>
        <!--  -->
        </ol>
    </answer>
</exercise>
