<exercise checkit-seed="0005" checkit-slug="Extra2" checkit-title="Clontz Spring 2022 Final">
    <statement>
        <p>
For each of the following ODEs, demonstrate how to find a
general solution (implicit or explicit). If initial value(s) are
given, also show how to find the corresponding particular solution.
        </p>
        <ol>
        <!--  -->
            <li>
                <p>
                    <m>-2 \, {y'} + {y''} + 14 \, e^{\left(5 \, t\right)} + 24 = 8 \, {y}</m>
                    <!--  -->
                    <!--  -->
                </p>
            </li>
        <!--  -->
            <li>
                <p>
                    <m>0 = 2 \, {y} - {y'} + 3 \, \delta\left(t - 5\right)</m>
                    <!--  -->
                    , <m>\,\,y(0) = 4</m>
                    <!--  -->
                    <!--  -->
                </p>
            </li>
        <!--  -->
            <li>
                <p>
                    <m>12 \, \cos\left(2 \, t\right) e^{\left(5 \, t\right)} - 2 \, {y'} = -10 \, {y}</m>
                    <!--  -->
                    , <m>\,\,y(0) = -4</m>
                    <!--  -->
                    <!--  -->
                </p>
            </li>
        <!--  -->
            <li>
                <p>
                    <m>-{y'} t + 3 \, {y} - 4 \, t = 0</m>
                    <!--  -->
                    , <m>\,\,y(-1) = -1</m>
                    <!--  -->
                    <!--  -->
                </p>
            </li>
        <!--  -->
            <li>
                <p>
                    <m>-4 \, {y'} = 12 \, {y}</m>
                    <!--  -->
                    , <m>\,\,y(\log\left(3\right)) = -\frac{4}{27}</m>
                    <!--  -->
                    <!--  -->
                </p>
            </li>
        <!--  -->
            <li>
                <p>
                    <m>6 \, {x} = -{x''} - 5 \, {x'}</m>
                    <!--  -->
                    , <m>\,\,y(0) = -5</m>
                    <!--  -->
                    <!--  -->
                    , <m>\,\,y'(0) = 13</m>
                    <!--  -->
                </p>
            </li>
        <!--  -->
            <li>
                <p>
                    <m>0 = -2 \, t y {y'} + 12 \, y^{2} {y'} - y^{2} + 5 \, t {y'} + 5 \, y</m>
                    <!--  -->
                    , <m>\,\,y(-1) = 1</m>
                    <!--  -->
                    <!--  -->
                </p>
            </li>
        <!--  -->
            <li>
                <p>
                    <m>100 \, {y} = -{y''}</m>
                    <!--  -->
                    , <m>\,\,y(0) = 4</m>
                    <!--  -->
                    <!--  -->
                    , <m>\,\,y'(0) = 50</m>
                    <!--  -->
                </p>
            </li>
        <!--  -->
        </ol>
    </statement>
    <answer>
        <ol>
        <!--  -->
            <li>
                <!--  -->
                <!--  -->
                <p>
                    <m>{y} = k_{1} e^{\left(4 \, t\right)} + k_{2} e^{\left(-2 \, t\right)} - 2 \, e^{\left(5 \, t\right)} + 3</m>
                </p>
                <!--  -->
            </li>
        <!--  -->
            <li>
                <!--  -->
                <p>
                    <m>{y} = 3 \, e^{\left(2 \, t - 10\right)} \mathrm{u}\left(t - 5\right) + 4 \, e^{\left(2 \, t\right)}</m>
                </p>
                <!--  -->
                <!--  -->
            </li>
        <!--  -->
            <li>
                <!--  -->
                <p>
                    <m>y = 3 \, e^{\left(5 \, t\right)} \sin\left(2 \, t\right) - 4 \, e^{\left(5 \, t\right)}</m>
                </p>
                <!--  -->
                <!--  -->
            </li>
        <!--  -->
            <li>
                <!--  -->
                <p>
                    <m>{y} = -t^{3} + 2 \, t</m>
                </p>
                <!--  -->
                <!--  -->
            </li>
        <!--  -->
            <li>
                <!--  -->
                <p>
                    <m>{y} = -4 \, e^{\left(-3 \, t\right)}</m>
                </p>
                <!--  -->
                <!--  -->
            </li>
        <!--  -->
            <li>
                <!--  -->
                <p>
                    <m>{x} = -2 \, e^{\left(-2 \, t\right)} - 3 \, e^{\left(-3 \, t\right)}</m>
                </p>
                <!--  -->
                <!--  -->
            </li>
        <!--  -->
            <li>
                <!--  -->
                <p>
                    <m>t y^{2} - 4 \, y^{3} - 5 \, t y = 0</m>
                </p>
                <!--  -->
                <!--  -->
            </li>
        <!--  -->
            <li>
                <!--  -->
                <p>
                    <m>{y} = 4 \, \cos\left(10 \, t\right) + 5 \, \sin\left(10 \, t\right)</m>
                </p>
                <!--  -->
                <!--  -->
            </li>
        <!--  -->
        </ol>
    </answer>
</exercise>
