<exercise checkit-seed="0006" checkit-slug="Extra2" checkit-title="Clontz Spring 2022 Final">
    <statement>
        <p>
For each of the following ODEs, demonstrate how to find a
general solution (implicit or explicit). If initial value(s) are
given, also show how to find the corresponding particular solution.
        </p>
        <ol>
        <!--  -->
            <li>
                <p>
                    <m>t {y'} + 3 \, {y} = -14 \, t^{4}</m>
                    <!--  -->
                    , <m>\,\,y(1) = -4</m>
                    <!--  -->
                    <!--  -->
                </p>
            </li>
        <!--  -->
            <li>
                <p>
                    <m>-3 \, {y'} = -9 \, {y}</m>
                    <!--  -->
                    , <m>\,\,y(\log\left(3\right)) = -108</m>
                    <!--  -->
                    <!--  -->
                </p>
            </li>
        <!--  -->
            <li>
                <p>
                    <m>4 \, {y} = -24 \, \cos\left(2 \, t\right) e^{t} + 4 \, {y'}</m>
                    <!--  -->
                    , <m>\,\,y(0) = 4</m>
                    <!--  -->
                    <!--  -->
                </p>
            </li>
        <!--  -->
            <li>
                <p>
                    <m>-5 \, e^{\left(2 \, t\right)} + 6 = -3 \, {y} + 2 \, {y'} + {y''}</m>
                    <!--  -->
                    <!--  -->
                </p>
            </li>
        <!--  -->
            <li>
                <p>
                    <m>-12 \, y^{3} {y'} + 2 \, t = -3 \, t {y'} - 3 \, y</m>
                    <!--  -->
                    , <m>\,\,y(-1) = 1</m>
                    <!--  -->
                    <!--  -->
                </p>
            </li>
        <!--  -->
            <li>
                <p>
                    <m>-{x''} - 16 \, {x} = 0</m>
                    <!--  -->
                    , <m>\,\,y(0) = -4</m>
                    <!--  -->
                    <!--  -->
                    , <m>\,\,y'(0) = 16</m>
                    <!--  -->
                </p>
            </li>
        <!--  -->
            <li>
                <p>
                    <m>5 \, {y} + {y'} - 2 \, \delta\left(t - 4\right) = 0</m>
                    <!--  -->
                    , <m>\,\,y(0) = 3</m>
                    <!--  -->
                    <!--  -->
                </p>
            </li>
        <!--  -->
            <li>
                <p>
                    <m>-6 \, {y'} = -{y''} - 5 \, {y}</m>
                    <!--  -->
                    , <m>\,\,y(0) = 1</m>
                    <!--  -->
                    <!--  -->
                    , <m>\,\,y'(0) = 21</m>
                    <!--  -->
                </p>
            </li>
        <!--  -->
        </ol>
    </statement>
    <answer>
        <ol>
        <!--  -->
            <li>
                <!--  -->
                <p>
                    <m>{y} = -2 \, t^{4} - \frac{2}{t^{3}}</m>
                </p>
                <!--  -->
                <!--  -->
            </li>
        <!--  -->
            <li>
                <!--  -->
                <p>
                    <m>{y} = -4 \, e^{\left(3 \, t\right)}</m>
                </p>
                <!--  -->
                <!--  -->
            </li>
        <!--  -->
            <li>
                <!--  -->
                <p>
                    <m>y = 3 \, e^{t} \sin\left(2 \, t\right) + 4 \, e^{t}</m>
                </p>
                <!--  -->
                <!--  -->
            </li>
        <!--  -->
            <li>
                <!--  -->
                <!--  -->
                <p>
                    <m>{y} = k_{1} e^{\left(-3 \, t\right)} + k_{2} e^{t} - e^{\left(2 \, t\right)} - 2</m>
                </p>
                <!--  -->
            </li>
        <!--  -->
            <li>
                <!--  -->
                <p>
                    <m>3 \, y^{4} - t^{2} - 3 \, t y = 5</m>
                </p>
                <!--  -->
                <!--  -->
            </li>
        <!--  -->
            <li>
                <!--  -->
                <p>
                    <m>{x} = -4 \, \cos\left(4 \, t\right) + 4 \, \sin\left(4 \, t\right)</m>
                </p>
                <!--  -->
                <!--  -->
            </li>
        <!--  -->
            <li>
                <!--  -->
                <p>
                    <m>{y} = 2 \, e^{\left(-5 \, t + 20\right)} \mathrm{u}\left(t - 4\right) + 3 \, e^{\left(-5 \, t\right)}</m>
                </p>
                <!--  -->
                <!--  -->
            </li>
        <!--  -->
            <li>
                <!--  -->
                <p>
                    <m>{y} = 5 \, e^{\left(5 \, t\right)} - 4 \, e^{t}</m>
                </p>
                <!--  -->
                <!--  -->
            </li>
        <!--  -->
        </ol>
    </answer>
</exercise>
