<exercise checkit-seed="0008" checkit-slug="Extra2" checkit-title="Clontz Spring 2022 Final">
    <statement>
        <p>
For each of the following ODEs, demonstrate how to find a
general solution (implicit or explicit). If initial value(s) are
given, also show how to find the corresponding particular solution.
        </p>
        <ol>
        <!--  -->
            <li>
                <p>
                    <m>0 = {y'} t - 2 \, {y} - \frac{10}{t^{3}}</m>
                    <!--  -->
                    , <m>\,\,y(1) = 2</m>
                    <!--  -->
                    <!--  -->
                </p>
            </li>
        <!--  -->
            <li>
                <p>
                    <m>8 \, t^{2} y {y'} + 10 \, y {y'} = -8 \, t y^{2} - 2 \, t {y'} - 2 \, y</m>
                    <!--  -->
                    , <m>\,\,y(1) = -1</m>
                    <!--  -->
                    <!--  -->
                </p>
            </li>
        <!--  -->
            <li>
                <p>
                    <m>6 \, {y} = 2 \, {y'}</m>
                    <!--  -->
                    , <m>\,\,y(\log\left(3\right)) = -108</m>
                    <!--  -->
                    <!--  -->
                </p>
            </li>
        <!--  -->
            <li>
                <p>
                    <m>20 \, e^{t} \sin\left(5 \, t\right) + 2 \, {y} - 2 \, {y'} = 0</m>
                    <!--  -->
                    , <m>\,\,y(0) = -3</m>
                    <!--  -->
                    <!--  -->
                </p>
            </li>
        <!--  -->
            <li>
                <p>
                    <m>{y''} + 4 \, {y} = 0</m>
                    <!--  -->
                    , <m>\,\,y(0) = -2</m>
                    <!--  -->
                    <!--  -->
                    , <m>\,\,y'(0) = 2</m>
                    <!--  -->
                </p>
            </li>
        <!--  -->
            <li>
                <p>
                    <m>0 = -8 \, {x'} - 15 \, {x} - {x''}</m>
                    <!--  -->
                    , <m>\,\,y(0) = 1</m>
                    <!--  -->
                    <!--  -->
                    , <m>\,\,y'(0) = -3</m>
                    <!--  -->
                </p>
            </li>
        <!--  -->
            <li>
                <p>
                    <m>{y'} = -5 \, {y} + 3 \, \delta\left(t - 6\right)</m>
                    <!--  -->
                    , <m>\,\,y(0) = -4</m>
                    <!--  -->
                    <!--  -->
                </p>
            </li>
        <!--  -->
            <li>
                <p>
                    <m>5 \, {y'} + {y''} + 6 \, {y} - 60 \, e^{\left(3 \, t\right)} + 12 = 0</m>
                    <!--  -->
                    <!--  -->
                </p>
            </li>
        <!--  -->
        </ol>
    </statement>
    <answer>
        <ol>
        <!--  -->
            <li>
                <!--  -->
                <p>
                    <m>{y} = 4 \, t^{2} - \frac{2}{t^{3}}</m>
                </p>
                <!--  -->
                <!--  -->
            </li>
        <!--  -->
            <li>
                <!--  -->
                <p>
                    <m>-4 \, t^{2} y^{2} - 2 \, t y - 5 \, y^{2} = \left(-7\right)</m>
                </p>
                <!--  -->
                <!--  -->
            </li>
        <!--  -->
            <li>
                <!--  -->
                <p>
                    <m>{y} = -4 \, e^{\left(3 \, t\right)}</m>
                </p>
                <!--  -->
                <!--  -->
            </li>
        <!--  -->
            <li>
                <!--  -->
                <p>
                    <m>y = -2 \, \cos\left(5 \, t\right) e^{t} - e^{t}</m>
                </p>
                <!--  -->
                <!--  -->
            </li>
        <!--  -->
            <li>
                <!--  -->
                <p>
                    <m>{y} = -2 \, \cos\left(2 \, t\right) + \sin\left(2 \, t\right)</m>
                </p>
                <!--  -->
                <!--  -->
            </li>
        <!--  -->
            <li>
                <!--  -->
                <p>
                    <m>{x} = e^{\left(-3 \, t\right)}</m>
                </p>
                <!--  -->
                <!--  -->
            </li>
        <!--  -->
            <li>
                <!--  -->
                <p>
                    <m>{y} = 3 \, e^{\left(-5 \, t + 30\right)} \mathrm{u}\left(t - 6\right) - 4 \, e^{\left(-5 \, t\right)}</m>
                </p>
                <!--  -->
                <!--  -->
            </li>
        <!--  -->
            <li>
                <!--  -->
                <!--  -->
                <p>
                    <m>{y} = k_{1} e^{\left(-2 \, t\right)} + k_{2} e^{\left(-3 \, t\right)} + 2 \, e^{\left(3 \, t\right)} - 2</m>
                </p>
                <!--  -->
            </li>
        <!--  -->
        </ol>
    </answer>
</exercise>
