<exercise checkit-seed="0001" checkit-slug="Extra2" checkit-title="Clontz Spring 2022 Final">
    <statement>
        <p>
For each of the following ODEs, demonstrate how to find a
general solution (implicit or explicit). If initial value(s) are
given, also show how to find the corresponding particular solution.
        </p>
        <ol>
        <!--  -->
            <li>
                <p>
                    <m>-5 \, {y} + {y'} = 6 \, \delta\left(t - 2\right)</m>
                    <!--  -->
                    , <m>\,\,y(0) = 4</m>
                    <!--  -->
                    <!--  -->
                </p>
            </li>
        <!--  -->
            <li>
                <p>
                    <m>-6 \, {y} + 18 \, e^{\left(3 \, t\right)} - 6 = -{y''} - {y'}</m>
                    <!--  -->
                    <!--  -->
                </p>
            </li>
        <!--  -->
            <li>
                <p>
                    <m>0 = -20 \, {x} + {x'} + {x''}</m>
                    <!--  -->
                    , <m>\,\,y(0) = 4</m>
                    <!--  -->
                    <!--  -->
                    , <m>\,\,y'(0) = -29</m>
                    <!--  -->
                </p>
            </li>
        <!--  -->
            <li>
                <p>
                    <m>-4 \, {y} = {y''}</m>
                    <!--  -->
                    , <m>\,\,y(0) = 4</m>
                    <!--  -->
                    <!--  -->
                    , <m>\,\,y'(0) = -10</m>
                    <!--  -->
                </p>
            </li>
        <!--  -->
            <li>
                <p>
                    <m>-{y'} t = -5 \, {y} - \frac{9}{t^{4}}</m>
                    <!--  -->
                    , <m>\,\,y(1) = 2</m>
                    <!--  -->
                    <!--  -->
                </p>
            </li>
        <!--  -->
            <li>
                <p>
                    <m>4 \, {y} = 2 \, {y'}</m>
                    <!--  -->
                    , <m>\,\,y(\log\left(2\right)) = 8</m>
                    <!--  -->
                    <!--  -->
                </p>
            </li>
        <!--  -->
            <li>
                <p>
                    <m>-40 \, e^{\left(4 \, t\right)} \sin\left(5 \, t\right) - 4 \, {y'} = -16 \, {y}</m>
                    <!--  -->
                    , <m>\,\,y(0) = 3</m>
                    <!--  -->
                    <!--  -->
                </p>
            </li>
        <!--  -->
            <li>
                <p>
                    <m>12 \, y^{3} {y'} - t^{2} {y'} - 2 \, t y = 6 \, t^{2} y {y'} + 6 \, t y^{2}</m>
                    <!--  -->
                    , <m>\,\,y(1) = -1</m>
                    <!--  -->
                    <!--  -->
                </p>
            </li>
        <!--  -->
        </ol>
    </statement>
    <answer>
        <ol>
        <!--  -->
            <li>
                <!--  -->
                <p>
                    <m>{y} = 6 \, e^{\left(5 \, t - 10\right)} \mathrm{u}\left(t - 2\right) + 4 \, e^{\left(5 \, t\right)}</m>
                </p>
                <!--  -->
                <!--  -->
            </li>
        <!--  -->
            <li>
                <!--  -->
                <!--  -->
                <p>
                    <m>{y} = k_{2} e^{\left(2 \, t\right)} + k_{1} e^{\left(-3 \, t\right)} - 3 \, e^{\left(3 \, t\right)} - 1</m>
                </p>
                <!--  -->
            </li>
        <!--  -->
            <li>
                <!--  -->
                <p>
                    <m>{x} = -e^{\left(4 \, t\right)} + 5 \, e^{\left(-5 \, t\right)}</m>
                </p>
                <!--  -->
                <!--  -->
            </li>
        <!--  -->
            <li>
                <!--  -->
                <p>
                    <m>{y} = 4 \, \cos\left(2 \, t\right) - 5 \, \sin\left(2 \, t\right)</m>
                </p>
                <!--  -->
                <!--  -->
            </li>
        <!--  -->
            <li>
                <!--  -->
                <p>
                    <m>{y} = 3 \, t^{5} - \frac{1}{t^{4}}</m>
                </p>
                <!--  -->
                <!--  -->
            </li>
        <!--  -->
            <li>
                <!--  -->
                <p>
                    <m>{y} = 2 \, e^{\left(2 \, t\right)}</m>
                </p>
                <!--  -->
                <!--  -->
            </li>
        <!--  -->
            <li>
                <!--  -->
                <p>
                    <m>y = 2 \, \cos\left(5 \, t\right) e^{\left(4 \, t\right)} + e^{\left(4 \, t\right)}</m>
                </p>
                <!--  -->
                <!--  -->
            </li>
        <!--  -->
            <li>
                <!--  -->
                <p>
                    <m>-3 \, t^{2} y^{2} + 3 \, y^{4} - t^{2} y = 1</m>
                </p>
                <!--  -->
                <!--  -->
            </li>
        <!--  -->
        </ol>
    </answer>
</exercise>
