<exercise checkit-seed="0004" checkit-slug="Extra2" checkit-title="Clontz Spring 2022 Final">
    <statement>
        <p>
For each of the following ODEs, demonstrate how to find a
general solution (implicit or explicit). If initial value(s) are
given, also show how to find the corresponding particular solution.
        </p>
        <ol>
        <!--  -->
            <li>
                <p>
                    <m>-8 \, t y^{2} + 4 \, t y {y'} + 2 \, y^{2} = 8 \, t^{2} y {y'} - 3 \, t^{2} {y'} - 6 \, t y</m>
                    <!--  -->
                    , <m>\,\,y(1) = -1</m>
                    <!--  -->
                    <!--  -->
                </p>
            </li>
        <!--  -->
            <li>
                <p>
                    <m>18 \, e^{\left(-2 \, t\right)} \sin\left(2 \, t\right) + 6 \, {y} = -3 \, {y'}</m>
                    <!--  -->
                    , <m>\,\,y(0) = 7</m>
                    <!--  -->
                    <!--  -->
                </p>
            </li>
        <!--  -->
            <li>
                <p>
                    <m>8 \, {y} + 4 \, {y'} = 0</m>
                    <!--  -->
                    , <m>\,\,y(\log\left(2\right)) = -\frac{3}{4}</m>
                    <!--  -->
                    <!--  -->
                </p>
            </li>
        <!--  -->
            <li>
                <p>
                    <m>0 = 64 \, {y} + {y''}</m>
                    <!--  -->
                    , <m>\,\,y(0) = 5</m>
                    <!--  -->
                    <!--  -->
                    , <m>\,\,y'(0) = -40</m>
                    <!--  -->
                </p>
            </li>
        <!--  -->
            <li>
                <p>
                    <m>-{y''} = -{y} + 72 \, e^{\left(5 \, t\right)} - 1</m>
                    <!--  -->
                    <!--  -->
                </p>
            </li>
        <!--  -->
            <li>
                <p>
                    <m>-15 \, t^{3} + 2 \, {y} = -t {y'}</m>
                    <!--  -->
                    , <m>\,\,y(1) = -1</m>
                    <!--  -->
                    <!--  -->
                </p>
            </li>
        <!--  -->
            <li>
                <p>
                    <m>-2 \, {x'} = {x''} - 3 \, {x}</m>
                    <!--  -->
                    , <m>\,\,y(0) = 2</m>
                    <!--  -->
                    <!--  -->
                    , <m>\,\,y'(0) = -18</m>
                    <!--  -->
                </p>
            </li>
        <!--  -->
            <li>
                <p>
                    <m>{y'} = -3 \, {y} - 6 \, \delta\left(t - 4\right)</m>
                    <!--  -->
                    , <m>\,\,y(0) = -2</m>
                    <!--  -->
                    <!--  -->
                </p>
            </li>
        <!--  -->
        </ol>
    </statement>
    <answer>
        <ol>
        <!--  -->
            <li>
                <!--  -->
                <p>
                    <m>-4 \, t^{2} y^{2} + 3 \, t^{2} y + 2 \, t y^{2} = \left(-5\right)</m>
                </p>
                <!--  -->
                <!--  -->
            </li>
        <!--  -->
            <li>
                <!--  -->
                <p>
                    <m>y = 3 \, \cos\left(2 \, t\right) e^{\left(-2 \, t\right)} + 4 \, e^{\left(-2 \, t\right)}</m>
                </p>
                <!--  -->
                <!--  -->
            </li>
        <!--  -->
            <li>
                <!--  -->
                <p>
                    <m>{y} = -3 \, e^{\left(-2 \, t\right)}</m>
                </p>
                <!--  -->
                <!--  -->
            </li>
        <!--  -->
            <li>
                <!--  -->
                <p>
                    <m>{y} = 5 \, \cos\left(8 \, t\right) - 5 \, \sin\left(8 \, t\right)</m>
                </p>
                <!--  -->
                <!--  -->
            </li>
        <!--  -->
            <li>
                <!--  -->
                <!--  -->
                <p>
                    <m>{y} = k_{1} e^{\left(-t\right)} + k_{2} e^{t} - 3 \, e^{\left(5 \, t\right)} - 1</m>
                </p>
                <!--  -->
            </li>
        <!--  -->
            <li>
                <!--  -->
                <p>
                    <m>{y} = 3 \, t^{3} - \frac{4}{t^{2}}</m>
                </p>
                <!--  -->
                <!--  -->
            </li>
        <!--  -->
            <li>
                <!--  -->
                <p>
                    <m>{x} = 5 \, e^{\left(-3 \, t\right)} - 3 \, e^{t}</m>
                </p>
                <!--  -->
                <!--  -->
            </li>
        <!--  -->
            <li>
                <!--  -->
                <p>
                    <m>{y} = -6 \, e^{\left(-3 \, t + 12\right)} \mathrm{u}\left(t - 4\right) - 2 \, e^{\left(-3 \, t\right)}</m>
                </p>
                <!--  -->
                <!--  -->
            </li>
        <!--  -->
        </ol>
    </answer>
</exercise>
