<exercise checkit-seed="0009" checkit-slug="Extra2" checkit-title="Clontz Spring 2022 Final">
    <statement>
        <p>
For each of the following ODEs, demonstrate how to find a
general solution (implicit or explicit). If initial value(s) are
given, also show how to find the corresponding particular solution.
        </p>
        <ol>
        <!--  -->
            <li>
                <p>
                    <m>4 \, t^{2} {y'} - 8 \, t y {y'} - 9 \, t^{2} - 4 \, y^{2} = -8 \, t y</m>
                    <!--  -->
                    , <m>\,\,y(1) = -1</m>
                    <!--  -->
                    <!--  -->
                </p>
            </li>
        <!--  -->
            <li>
                <p>
                    <m>4 \, {y} + 5 \, {y'} = -{y''}</m>
                    <!--  -->
                    , <m>\,\,y(0) = 3</m>
                    <!--  -->
                    <!--  -->
                    , <m>\,\,y'(0) = -6</m>
                    <!--  -->
                </p>
            </li>
        <!--  -->
            <li>
                <p>
                    <m>3 \, {y} = {y'} + 5 \, \delta\left(t - 4\right)</m>
                    <!--  -->
                    , <m>\,\,y(0) = -2</m>
                    <!--  -->
                    <!--  -->
                </p>
            </li>
        <!--  -->
            <li>
                <p>
                    <m>-{y'} t + 5 \, {y} = \frac{7}{t^{2}}</m>
                    <!--  -->
                    , <m>\,\,y(-1) = -3</m>
                    <!--  -->
                    <!--  -->
                </p>
            </li>
        <!--  -->
            <li>
                <p>
                    <m>81 \, {x} = -{x''}</m>
                    <!--  -->
                    , <m>\,\,y(0) = 3</m>
                    <!--  -->
                    <!--  -->
                    , <m>\,\,y'(0) = -36</m>
                    <!--  -->
                </p>
            </li>
        <!--  -->
            <li>
                <p>
                    <m>4 \, {y'} = -12 \, {y}</m>
                    <!--  -->
                    , <m>\,\,y(\log\left(2\right)) = \frac{3}{8}</m>
                    <!--  -->
                    <!--  -->
                </p>
            </li>
        <!--  -->
            <li>
                <p>
                    <m>12 \, e^{\left(-t\right)} = -4 \, {y'} - 4 \, {y}</m>
                    <!--  -->
                    , <m>\,\,y(0) = 2</m>
                    <!--  -->
                    <!--  -->
                </p>
            </li>
        <!--  -->
            <li>
                <p>
                    <m>{y''} - {y'} + 8 \, e^{\left(2 \, t\right)} - 6 = 6 \, {y}</m>
                    <!--  -->
                    <!--  -->
                </p>
            </li>
        <!--  -->
        </ol>
    </statement>
    <answer>
        <ol>
        <!--  -->
            <li>
                <!--  -->
                <p>
                    <m>3 \, t^{3} - 4 \, t^{2} y + 4 \, t y^{2} = 11</m>
                </p>
                <!--  -->
                <!--  -->
            </li>
        <!--  -->
            <li>
                <!--  -->
                <p>
                    <m>{y} = 2 \, e^{\left(-t\right)} + e^{\left(-4 \, t\right)}</m>
                </p>
                <!--  -->
                <!--  -->
            </li>
        <!--  -->
            <li>
                <!--  -->
                <p>
                    <m>{y} = -5 \, e^{\left(3 \, t - 12\right)} \mathrm{u}\left(t - 4\right) - 2 \, e^{\left(3 \, t\right)}</m>
                </p>
                <!--  -->
                <!--  -->
            </li>
        <!--  -->
            <li>
                <!--  -->
                <p>
                    <m>{y} = 4 \, t^{5} + \frac{1}{t^{2}}</m>
                </p>
                <!--  -->
                <!--  -->
            </li>
        <!--  -->
            <li>
                <!--  -->
                <p>
                    <m>{x} = 3 \, \cos\left(9 \, t\right) - 4 \, \sin\left(9 \, t\right)</m>
                </p>
                <!--  -->
                <!--  -->
            </li>
        <!--  -->
            <li>
                <!--  -->
                <p>
                    <m>{y} = 3 \, e^{\left(-3 \, t\right)}</m>
                </p>
                <!--  -->
                <!--  -->
            </li>
        <!--  -->
            <li>
                <!--  -->
                <p>
                    <m>y = -3 \, t e^{\left(-t\right)} + 2 \, e^{\left(-t\right)}</m>
                </p>
                <!--  -->
                <!--  -->
            </li>
        <!--  -->
            <li>
                <!--  -->
                <!--  -->
                <p>
                    <m>{y} = k_{2} e^{\left(3 \, t\right)} + k_{1} e^{\left(-2 \, t\right)} + 2 \, e^{\left(2 \, t\right)} - 1</m>
                </p>
                <!--  -->
            </li>
        <!--  -->
        </ol>
    </answer>
</exercise>
