<exercise checkit-seed="0003" checkit-slug="Extra2" checkit-title="Clontz Spring 2022 Final">
    <statement>
        <p>
For each of the following ODEs, demonstrate how to find a
general solution (implicit or explicit). If initial value(s) are
given, also show how to find the corresponding particular solution.
        </p>
        <ol>
        <!--  -->
            <li>
                <p>
                    <m>{y''} + 2 \, {y'} - 8 \, {y} = -14 \, e^{\left(3 \, t\right)} + 24</m>
                    <!--  -->
                    <!--  -->
                </p>
            </li>
        <!--  -->
            <li>
                <p>
                    <m>-{y'} t - 3 \, {y} = 30 \, t^{3}</m>
                    <!--  -->
                    , <m>\,\,y(1) = -1</m>
                    <!--  -->
                    <!--  -->
                </p>
            </li>
        <!--  -->
            <li>
                <p>
                    <m>0 = -81 \, {y} - {y''}</m>
                    <!--  -->
                    , <m>\,\,y(0) = 0</m>
                    <!--  -->
                    <!--  -->
                    , <m>\,\,y'(0) = -45</m>
                    <!--  -->
                </p>
            </li>
        <!--  -->
            <li>
                <p>
                    <m>4 \, {y'} - 12 \, {y} = 8 \, e^{\left(3 \, t\right)}</m>
                    <!--  -->
                    , <m>\,\,y(0) = 4</m>
                    <!--  -->
                    <!--  -->
                </p>
            </li>
        <!--  -->
            <li>
                <p>
                    <m>8 \, t y^{2} + 4 \, t y {y'} + 2 \, y^{2} = -8 \, t^{2} y {y'} - 12 \, y^{2} {y'}</m>
                    <!--  -->
                    , <m>\,\,y(-1) = 1</m>
                    <!--  -->
                    <!--  -->
                </p>
            </li>
        <!--  -->
            <li>
                <p>
                    <m>3 \, {y'} = 9 \, {y}</m>
                    <!--  -->
                    , <m>\,\,y(\log\left(2\right)) = -24</m>
                    <!--  -->
                    <!--  -->
                </p>
            </li>
        <!--  -->
            <li>
                <p>
                    <m>-4 \, {y} - {y'} - 5 \, \delta\left(t - 6\right) = 0</m>
                    <!--  -->
                    , <m>\,\,y(0) = -2</m>
                    <!--  -->
                    <!--  -->
                </p>
            </li>
        <!--  -->
            <li>
                <p>
                    <m>-{x''} + 4 \, {x} = 3 \, {x'}</m>
                    <!--  -->
                    , <m>\,\,y(0) = 8</m>
                    <!--  -->
                    <!--  -->
                    , <m>\,\,y'(0) = -7</m>
                    <!--  -->
                </p>
            </li>
        <!--  -->
        </ol>
    </statement>
    <answer>
        <ol>
        <!--  -->
            <li>
                <!--  -->
                <!--  -->
                <p>
                    <m>{y} = k_{2} e^{\left(2 \, t\right)} + k_{1} e^{\left(-4 \, t\right)} - 2 \, e^{\left(3 \, t\right)} - 3</m>
                </p>
                <!--  -->
            </li>
        <!--  -->
            <li>
                <!--  -->
                <p>
                    <m>{y} = -5 \, t^{3} + \frac{4}{t^{3}}</m>
                </p>
                <!--  -->
                <!--  -->
            </li>
        <!--  -->
            <li>
                <!--  -->
                <p>
                    <m>{y} = -5 \, \sin\left(9 \, t\right)</m>
                </p>
                <!--  -->
                <!--  -->
            </li>
        <!--  -->
            <li>
                <!--  -->
                <p>
                    <m>y = 2 \, t e^{\left(3 \, t\right)} + 4 \, e^{\left(3 \, t\right)}</m>
                </p>
                <!--  -->
                <!--  -->
            </li>
        <!--  -->
            <li>
                <!--  -->
                <p>
                    <m>4 \, t^{2} y^{2} + 2 \, t y^{2} + 4 \, y^{3} = 6</m>
                </p>
                <!--  -->
                <!--  -->
            </li>
        <!--  -->
            <li>
                <!--  -->
                <p>
                    <m>{y} = -3 \, e^{\left(3 \, t\right)}</m>
                </p>
                <!--  -->
                <!--  -->
            </li>
        <!--  -->
            <li>
                <!--  -->
                <p>
                    <m>{y} = -5 \, e^{\left(-4 \, t + 24\right)} \mathrm{u}\left(t - 6\right) - 2 \, e^{\left(-4 \, t\right)}</m>
                </p>
                <!--  -->
                <!--  -->
            </li>
        <!--  -->
            <li>
                <!--  -->
                <p>
                    <m>{x} = 3 \, e^{\left(-4 \, t\right)} + 5 \, e^{t}</m>
                </p>
                <!--  -->
                <!--  -->
            </li>
        <!--  -->
        </ol>
    </answer>
</exercise>
