<exercise checkit-seed="0002" checkit-slug="Extra2" checkit-title="Clontz Spring 2022 Final">
    <statement>
        <p>
For each of the following ODEs, demonstrate how to find a
general solution (implicit or explicit). If initial value(s) are
given, also show how to find the corresponding particular solution.
        </p>
        <ol>
        <!--  -->
            <li>
                <p>
                    <m>6 \, {y} + {y'} = -2 \, \delta\left(t - 3\right)</m>
                    <!--  -->
                    , <m>\,\,y(0) = -4</m>
                    <!--  -->
                    <!--  -->
                </p>
            </li>
        <!--  -->
            <li>
                <p>
                    <m>4 \, {x} + 3 \, {x'} = {x''}</m>
                    <!--  -->
                    , <m>\,\,y(0) = -2</m>
                    <!--  -->
                    <!--  -->
                    , <m>\,\,y'(0) = -18</m>
                    <!--  -->
                </p>
            </li>
        <!--  -->
            <li>
                <p>
                    <m>0 = -6 \, {y} + 3 \, {y'}</m>
                    <!--  -->
                    , <m>\,\,y(\log\left(3\right)) = 18</m>
                    <!--  -->
                    <!--  -->
                </p>
            </li>
        <!--  -->
            <li>
                <p>
                    <m>0 = -16 \, t^{3} - 3 \, t^{2} {y'} - 6 \, t y - t {y'} - y</m>
                    <!--  -->
                    , <m>\,\,y(1) = -1</m>
                    <!--  -->
                    <!--  -->
                </p>
            </li>
        <!--  -->
            <li>
                <p>
                    <m>{y''} + 36 \, {y} = 0</m>
                    <!--  -->
                    , <m>\,\,y(0) = 1</m>
                    <!--  -->
                    <!--  -->
                    , <m>\,\,y'(0) = 18</m>
                    <!--  -->
                </p>
            </li>
        <!--  -->
            <li>
                <p>
                    <m>12 \, \cos\left(2 \, t\right) e^{\left(-2 \, t\right)} = -2 \, {y'} - 4 \, {y}</m>
                    <!--  -->
                    , <m>\,\,y(0) = 1</m>
                    <!--  -->
                    <!--  -->
                </p>
            </li>
        <!--  -->
            <li>
                <p>
                    <m>-4 \, {y} + \frac{24}{t^{4}} = -{y'} t</m>
                    <!--  -->
                    , <m>\,\,y(-1) = 2</m>
                    <!--  -->
                    <!--  -->
                </p>
            </li>
        <!--  -->
            <li>
                <p>
                    <m>0 = 3 \, {y} + {y''} - 4 \, {y'} + 3 \, e^{\left(2 \, t\right)} + 3</m>
                    <!--  -->
                    <!--  -->
                </p>
            </li>
        <!--  -->
        </ol>
    </statement>
    <answer>
        <ol>
        <!--  -->
            <li>
                <!--  -->
                <p>
                    <m>{y} = -2 \, e^{\left(-6 \, t + 18\right)} \mathrm{u}\left(t - 3\right) - 4 \, e^{\left(-6 \, t\right)}</m>
                </p>
                <!--  -->
                <!--  -->
            </li>
        <!--  -->
            <li>
                <!--  -->
                <p>
                    <m>{x} = -4 \, e^{\left(4 \, t\right)} + 2 \, e^{\left(-t\right)}</m>
                </p>
                <!--  -->
                <!--  -->
            </li>
        <!--  -->
            <li>
                <!--  -->
                <p>
                    <m>{y} = 2 \, e^{\left(2 \, t\right)}</m>
                </p>
                <!--  -->
                <!--  -->
            </li>
        <!--  -->
            <li>
                <!--  -->
                <p>
                    <m>-4 \, t^{4} - 3 \, t^{2} y - t y = 0</m>
                </p>
                <!--  -->
                <!--  -->
            </li>
        <!--  -->
            <li>
                <!--  -->
                <p>
                    <m>{y} = \cos\left(6 \, t\right) + 3 \, \sin\left(6 \, t\right)</m>
                </p>
                <!--  -->
                <!--  -->
            </li>
        <!--  -->
            <li>
                <!--  -->
                <p>
                    <m>y = -3 \, e^{\left(-2 \, t\right)} \sin\left(2 \, t\right) + e^{\left(-2 \, t\right)}</m>
                </p>
                <!--  -->
                <!--  -->
            </li>
        <!--  -->
            <li>
                <!--  -->
                <p>
                    <m>{y} = -t^{4} + \frac{3}{t^{4}}</m>
                </p>
                <!--  -->
                <!--  -->
            </li>
        <!--  -->
            <li>
                <!--  -->
                <!--  -->
                <p>
                    <m>{y} = k_{2} e^{\left(3 \, t\right)} + k_{1} e^{t} + 3 \, e^{\left(2 \, t\right)} - 1</m>
                </p>
                <!--  -->
            </li>
        <!--  -->
        </ol>
    </answer>
</exercise>
